chore: rename TC to Relation.TransGen (#4760)
This is barely used in Lean, and this rename is both more readable, and
consistent with further developments downstream.

See
[zulip](https://leanprover.zulipchat.com/#narrow/stream/287929-mathlib4/topic/Relation.2ETransGen.20vs.2E.20TC.20from.20Init.2ECore/near/448941824)
discussion.

src/Init/WF.lean
@@ -148,22 +148,26 @@ end InvImage
   wf  := InvImage.wf f h.wf
 
 -- The transitive closure of a well-founded relation is well-founded
-namespace TC
-variable {α : Sort u} {r : α → α → Prop}
+open Relation
 
-theorem accessible {z : α} (ac : Acc r z) : Acc (TC r) z := by
-  induction ac with
-  | intro x acx ih =>
-    apply Acc.intro x
-    intro y rel
-    induction rel with
-    | base a b rab => exact ih a rab
-    | trans a b c rab _ _ ih₂ => apply Acc.inv (ih₂ acx ih) rab
+theorem Acc.transGen (h : Acc r a) : Acc (TransGen r) a := by
+  induction h with
+  | intro x _ H =>
+    refine Acc.intro x fun y hy ↦ ?_
+    cases hy with
+    | single hyx =>
+      exact H y hyx
+    | tail hyz hzx =>
+      exact (H _ hzx).inv hyz
 
-theorem wf (h : WellFounded r) : WellFounded (TC r) :=
-  ⟨fun a => accessible (apply h a)⟩
-end TC
+theorem acc_transGen_iff : Acc (TransGen r) a ↔ Acc r a :=
+  ⟨Subrelation.accessible TransGen.single, Acc.transGen⟩
 
+theorem WellFounded.transGen (h : WellFounded r) : WellFounded (TransGen r) :=
+  ⟨fun a ↦ (h.apply a).transGen⟩
+
+@[deprecated Acc.transGen (since := "2024-07-16")] abbrev TC.accessible := @Acc.transGen
+@[deprecated WellFounded.transGen (since := "2024-07-16")] abbrev TC.wf := @WellFounded.transGen
 namespace Nat
 
 -- less-than is well-founded
